Implement between-section jump removal
The main optimisation required for lab_simp is not the within-section
version (already verified); this commit adds the between-section version
(with no proofs). Also, rename and update the existing proof of the
within-section version. Also simplify it to not delete empty sections
(which are assumed not to occur anyway).

compiler/backend/lab_simpScript.sml
@@ -2,21 +2,39 @@ open preamble labLangTheory;
 
 val _ = new_theory "lab_simp";
 
-val lab_simp_sec_def = Define `
-(lab_simp_sec (a :: b :: xs) =
+val lab_simp_lines_def = Define `
+(lab_simp_lines (a :: b :: xs) =
  case (a, b) of
    | ((LabAsm (Jump (Lab n11 n21)) w wl n), (Label n12 n22 k))
-     => if (n11 = n12 /\ n21 = n22) then (Asm (Inst Skip) wl n :: Label n12 n22 k :: lab_simp_sec xs) else (a :: b :: lab_simp_sec xs)
-   | _ => a :: b :: lab_simp_sec xs) /\
-(lab_simp_sec x = x)
-`;
+     => if (n11 = n12 /\ n21 = n22) then (Asm (Inst Skip) wl n :: Label n12 n22 k :: lab_simp_lines xs) else (a :: b :: lab_simp_lines xs)
+   | _ => a :: b :: lab_simp_lines xs) /\
+(lab_simp_lines x = x)`;
+
+val lab_simp_sec_def = Define`
+  lab_simp_sec (Section k ls) = Section k (lab_simp_lines ls)`;
+val _ = export_rewrites["lab_simp_sec_def"];
+
+val has_last_jump_def = Define`
+  (has_last_jump k i [] ⇔ NONE) ∧
+  (has_last_jump k i (x::xs) ⇔
+    case x of
+    | (LabAsm (Jump k') _ wl n) =>
+      if k = k' ∧ EVERY (λx. is_Label x ∨ is_Skip x) xs then SOME (i,wl,n)
+      else has_last_jump k (i+1n) xs
+    | _ => has_last_jump k (i+1n) xs)`;
+
+val replace_last_jump_def = Define`
+  replace_last_jump k ls =
+    case has_last_jump (Lab k 0) 0 ls of NONE => ls
+    | SOME (i,wl,n) => LUPDATE (Asm (Inst Skip) wl n) i ls`;
+
+val remove_tail_jumps_def = Define`
+  (remove_tail_jumps [] = []) ∧
+  (remove_tail_jumps [s] = [s]) ∧
+  (remove_tail_jumps (Section k1 l1::(Section k2 l2::ss)) =
+   Section k1 (replace_last_jump k2 l1)::remove_tail_jumps (Section k2 l2::ss))`;
 
 val lab_simp_def = Define `
-(lab_simp ((Section k lines) :: sections) =
- let simpd = lab_simp_sec lines in
-     if NULL simpd
-     then lab_simp sections
-     else (Section k simpd) :: lab_simp sections) /\
-(lab_simp [] = [])`;
+  lab_simp ss = remove_tail_jumps (MAP lab_simp_sec ss)`;
 
 val _ = export_theory ();
